\documentclass[preview]{standalone}

\usepackage[english]{babel}
\usepackage{amsmath}
\usepackage{amssymb}

\begin{document}

\begin{center}
Evaluando los t√©rminos de la anterior sumatoria tenemos:

(n = 0):
$$ \frac{(i\theta)^0}{0!} = 1 $$

(n = 1):
$$ \frac{(i\theta)^1}{1!} = i\theta $$

(n = 2):
$$ \frac{(i\theta)^2}{2!} = -\frac{\theta^2}{2} $$

(n = 3):
$$ \frac{(i\theta)^3}{3!} = -\frac{i\theta^3}{6} $$

(n = 4):
$$ \frac{(i\theta)^4}{4!} = \frac{\theta^4}{24} $$
\end{center}

\end{document}
